@prefix : <http://w3id.org/medred/medred#> .
@prefix dc: <http://purl.org/dc/elements/1.1/> .
@prefix sh: <http://www.w3.org/ns/shacl#> .
@prefix owl: <http://www.w3.org/2002/07/owl#> .
@prefix rdf: <http://www.w3.org/1999/02/22-rdf-syntax-ns#> .
@prefix xml: <http://www.w3.org/XML/1998/namespace> .
@prefix xsd: <http://www.w3.org/2001/XMLSchema#> .
@prefix prov: <http://www.w3.org/ns/prov#> .
@prefix rdfs: <http://www.w3.org/2000/01/rdf-schema#> .
@prefix disco: <http://rdf-vocabulary.ddialliance.org/discovery#> .
@prefix p-plan: <http://purl.org/net/p-plan#> .
@prefix dcterms: <http://purl.org/dc/terms/> .

<http://w3id.org/medred/medred#> a owl:Ontology ;
	owl:imports <http://rdf-vocabulary.ddialliance.org/discovery> , <http://purl.org/net/p-plan#> ;
	dcterms:modified "2017-04-25"^^xsd:date ;
	dc:publisher <http://aislab.hevs.ch/> ;
	dcterms:rights "Copyright © 2017 HES-SO Valais-Wallis" ;
	<http://purl.org/vocab/vann/preferredNamespacePrefix> "medred" ;
	dcterms:description "Esta ontología has sido diseñada para representar Instrumentos de captura de datos clínicos, dentro del contexto del proyecto MedRed (https://www.hevs.ch/en/rad-institutes/institute-of-information-systems/projects/medical-research-data-acquisition-platform-14092)"@es ;
	dcterms:title "MedRed ontology: clinical data acquisition model"@en ;
	dcterms:creator <http://w3id.org/people/jpcik/me> ;
	owl:versionInfo "0.0.1" ;
	dcterms:issued "2017-04-01"^^xsd:date ;
	dcterms:publisher <http://w3id.org/hes-so/aislab> ;
	dcterms:license <https://creativecommons.org/licenses/by/4.0/> ;
	<http://purl.org/vocab/vann/preferredNamespaceUri> "http://w3id.org/medred/medred#" ;
	dcterms:title "Ontología MedRed: modelo de adquisición de datos clínicos"@es ;
	dcterms:description "This ontology aims to model generic Medical Data Acquisition Instruments, which can be interoperable across different clinical data management systems. The ontology is developed in the context of the MedRed project (https://www.hevs.ch/en/rad-institutes/institute-of-information-systems/projects/medical-research-data-acquisition-platform-14092)"@en ;
	rdfs:comment "Esta ontología has sido diseñada para representar Instrumentos de captura de datos clínicos, dentro del contexto del proyecto MedRed (https://www.hevs.ch/en/rad-institutes/institute-of-information-systems/projects/medical-research-data-acquisition-platform-14092)"@es ;
	dcterms:title "MedRed ontologie: modèle d'aquisition de données cliniques"@fr ;
	rdfs:comment "This ontology aims to model generic Medical Data Acquisition Instruments, which can be interoperable across different clinical data management systems. The ontology is developed in the context of the MedRed project (https://www.hevs.ch/en/rad-institutes/institute-of-information-systems/projects/medical-research-data-acquisition-platform-14092)"@en , "Cette ontologie a été conçue pour representer des Instruments pour l'aquisition de données cliniques, dans le contexte du projet MedRed project (https://www.hevs.ch/en/rad-institutes/institute-of-information-systems/projects/medical-research-data-acquisition-platform-14092)"@fr ;
	dcterms:description "Cette ontologie a été conçue pour representer des Instruments pour l'aquisition de données cliniques, dans le contexte du projet MedRed project (https://www.hevs.ch/en/rad-institutes/institute-of-information-systems/projects/medical-research-data-acquisition-platform-14092)"@fr .
# 
# 
# #################################################################
# #
# #    Object Properties
# #
# #################################################################
# 
# 
# http://w3id.org/medred/medred#dataType

:dataType a owl:ObjectProperty ;
	rdfs:subPropertyOf owl:topObjectProperty ;
	rdfs:domain p-plan:Variable ;
	rdfs:range rdfs:Datatype ;
	rdfs:comment "The dataType estalbishes a relationship between a Variable and the datatype of its data item"@en ;
	rdfs:isDefinedBy <http://w3id.org/medred/medred#> ;
	rdfs:label "dataType"@en .
# 
# http://w3id.org/medred/medred#hasArms

:hasArms a owl:ObjectProperty ;
	rdfs:domain :Study ;
	rdfs:range :ArmList ;
	rdfs:comment "A relation between a Study and a list of its different Arms"@en ;
	rdfs:isDefinedBy <http://w3id.org/medred/medred#> ;
	rdfs:label "hasArms"@en ;
	rdfs:seeAlso :Arm , :Study .
# 
# http://w3id.org/medred/medred#hasChoices

:hasChoices a owl:ObjectProperty ;
	rdfs:domain :Question ;
	rdfs:range :ChoiceList ;
	rdfs:comment "A relation between an Instrument question, and the list of possible Choice elements"@en ;
	rdfs:isDefinedBy <http://w3id.org/medred/medred#> ;
	rdfs:label "hasChoices"@en ;
	rdfs:seeAlso :Choice .
# 
# http://w3id.org/medred/medred#hasInstruments

:hasInstruments a owl:ObjectProperty ;
	rdfs:domain :Study ;
	rdfs:range :InstrumentList ;
	rdfs:comment "The instrument establishes a relationship between a Study and a list of Instruments"@en ;
	rdfs:isDefinedBy <http://w3id.org/medred/medred#> ;
	rdfs:label "hasInstruments"@en ;
	rdfs:seeAlso :Instrument .
# 
# http://w3id.org/medred/medred#includedInStudy

:includedInStudy a owl:ObjectProperty ;
	rdfs:domain _:genid1 .

_:genid1 a owl:Class ;
	owl:unionOf _:genid3 .

_:genid3 a rdf:List ;
	rdf:first :Arm ;
	rdf:rest _:genid2 .

_:genid2 a rdf:List ;
	rdf:first :Instrument ;
	rdf:rest rdf:nil .

:includedInStudy rdfs:range :Study ;
	rdfs:comment "It establishes a relationship between an Arm or Instrument, and a Study"@en ;
	rdfs:isDefinedBy <http://w3id.org/medred/medred#> ;
	rdfs:label "includedInStudy"@en ;
	rdfs:seeAlso :Arm , :Instrument , :Study .
# 
# http://w3id.org/medred/medred#includesEvents

:includesEvents a owl:ObjectProperty ;
	rdfs:domain _:genid4 .

_:genid4 a owl:Class ;
	owl:unionOf _:genid6 .

_:genid6 a rdf:List ;
	rdf:first :Arm ;
	rdf:rest _:genid5 .

_:genid5 a rdf:List ;
	rdf:first :Study ;
	rdf:rest rdf:nil .

:includesEvents rdfs:range :EventList ;
	rdfs:comment "A relation between an Arm or Study, and the list of its events"@en ;
	rdfs:isDefinedBy <http://w3id.org/medred/medred#> ;
	rdfs:label "includesEvents"@en ;
	rdfs:seeAlso :Arm , :StudyEvent .
# 
# http://w3id.org/medred/medred#includesInstrument

:includesInstrument a owl:ObjectProperty ;
	rdfs:domain :StudyEvent ;
	rdfs:range :Instrument ;
	rdfs:comment "A relation between an StudyEvent, and an Instrument it includes"@en ;
	rdfs:isDefinedBy <http://w3id.org/medred/medred#> ;
	rdfs:label "includesInstrument"@en ;
	rdfs:seeAlso :Instrument , :StudyEvent .
# 
# http://w3id.org/medred/medred#isEventOfArm

:isEventOfArm a owl:ObjectProperty ;
	rdfs:domain :StudyEvent ;
	rdfs:range :Arm ;
	rdfs:comment "It establishes a relationship between a StudyEvent, and an Arm"@en ;
	rdfs:isDefinedBy <http://w3id.org/medred/medred#> ;
	rdfs:label "isEventOfArm"@en ;
	rdfs:seeAlso :Arm , :StudyEvent .
# 
# http://w3id.org/medred/medred#isItemOfInstrument

:isItemOfInstrument a owl:ObjectProperty ;
	rdfs:subPropertyOf p-plan:isStepOfPlan ;
	rdfs:domain :Item ;
	rdfs:range :Instrument ;
	rdfs:comment "It establishes a relationship between an Item and an Instrument"@en ;
	rdfs:isDefinedBy <http://w3id.org/medred/medred#> ;
	rdfs:label "isItemofInstrument"@en ;
	rdfs:seeAlso :Instrument , :Item .
# 
# http://w3id.org/medred/medred#isItemOfSection

:isItemOfSection a owl:ObjectProperty ;
	rdfs:subPropertyOf p-plan:isStepOfPlan ;
	rdfs:domain :Item ;
	rdfs:range :Section ;
	rdfs:comment "It establishes a relationship between an Item and a Section"@en ;
	rdfs:isDefinedBy <http://w3id.org/medred/medred#> ;
	rdfs:label "isItemofSection"@en ;
	rdfs:seeAlso :Item , :Section .
# 
# http://w3id.org/medred/medred#items

:items a owl:ObjectProperty ;
	rdfs:domain _:genid7 .

_:genid7 a owl:Class ;
	owl:unionOf _:genid9 .

_:genid9 a rdf:List ;
	rdf:first :Instrument ;
	rdf:rest _:genid8 .

_:genid8 a rdf:List ;
	rdf:first :Item ;
	rdf:rest rdf:nil .

:items rdfs:range :ItemList ;
	rdfs:comment "The items property represents a relationship between an Instrument and its constitutent ItemList"@en ;
	rdfs:isDefinedBy <http://w3id.org/medred/medred#> ;
	rdfs:label "items"@en ;
	rdfs:seeAlso :ItemList .
# 
# http://w3id.org/medred/medred#validationShape

:validationShape a owl:ObjectProperty ;
	rdfs:domain :Item ;
	rdfs:range sh:PropertyShape ;
	rdfs:comment "It establishes a relationship between an Item, and a PropertyShape, which defines the type of validation expected for the Observations made for the Item."@en ;
	rdfs:isDefinedBy <http://w3id.org/medred/medred#> ;
	rdfs:label "validationShape"@en ;
	rdfs:seeAlso :Item , sh:PropertyShape .
# 
# http://www.w3.org/1999/02/22-rdf-syntax-ns#first

rdf:first a owl:ObjectProperty .
# 
# http://www.w3.org/1999/02/22-rdf-syntax-ns#rest

rdf:rest a owl:ObjectProperty .
# 
# 
# 
# #################################################################
# #
# #    Data properties
# #
# #################################################################
# 
# 
# http://purl.org/dc/terms/title

dcterms:title a owl:DatatypeProperty .
# 
# http://w3id.org/medred/medred#calculation

:calculation a owl:DatatypeProperty ;
	rdfs:domain :Operation ;
	rdfs:range rdfs:Literal ;
	rdfs:comment "It indicates the definition of a calculation or a computation on an Operation item, over input variables."@en ;
	rdfs:isDefinedBy <http://w3id.org/medred/medred#> ;
	rdfs:label "calculation"@en ;
	rdfs:seeAlso :Operation .
# 
# http://w3id.org/medred/medred#dataValue

:dataValue a owl:DatatypeProperty ;
	rdfs:domain :Observation ;
	rdfs:range rdfs:Literal ;
	rdfs:comment "It establishes a value of a data element related to a given Observation"@en ;
	rdfs:isDefinedBy <http://w3id.org/medred/medred#> ;
	rdfs:label "dataValue"@en .
# 
# http://w3id.org/medred/medred#hasValue

:hasValue a owl:DatatypeProperty ;
	rdfs:domain :Choice ;
	rdfs:range rdfs:Literal ;
	rdfs:comment "It establishes a value for a given Choice element."@en ;
	rdfs:isDefinedBy <http://w3id.org/medred/medred#> ;
	rdfs:label "hasValue"@en .
# 
# http://w3id.org/medred/medred#studyName

:studyName a owl:DatatypeProperty ;
	rdfs:subPropertyOf dcterms:title ;
	rdfs:domain :Study ;
	rdfs:range xsd:string ;
	rdfs:comment "It establishes a value for the name of the study"@en ;
	rdfs:isDefinedBy <http://w3id.org/medred/medred#> ;
	rdfs:label "studyName"@en .
# 
# http://w3id.org/medred/medred#varName

:varName a owl:DatatypeProperty ;
	rdfs:domain p-plan:Variable ;
	rdfs:range xsd:string ;
	rdfs:comment "It establishes a value for the name of a Variable"@en ;
	rdfs:isDefinedBy <http://w3id.org/medred/medred#> ;
	rdfs:label "varName"@en .
# 
# 
# 
# #################################################################
# #
# #    Classes
# #
# #################################################################
# 
# 
# http://purl.org/vocommons/voaf#Vocabulary

<http://purl.org/vocommons/voaf#Vocabulary> a owl:Class .
# 
# http://w3id.org/medred/medred#Arm

:Arm a owl:Class ;
	rdfs:subClassOf p-plan:Plan ;
	owl:disjointWith :Instrument ;
	rdfs:comment "An Arm is branching of a study that corresponds to a particular set of conditions, typically used to compare different behaviours, patterns or steps within the same study. Different Arms typically will have different sets of Instruments applied over time."@en ;
	rdfs:isDefinedBy <http://w3id.org/medred/medred#> ;
	rdfs:label "Arm"@en ;
	rdfs:seeAlso :Instrument , :Study .
# 
# http://w3id.org/medred/medred#ArmList

:ArmList a owl:Class ;
	rdfs:subClassOf rdf:List ;
	rdfs:comment "A ArmList is an ordered sequence of Arms, for a given study."@en ;
	rdfs:isDefinedBy <http://w3id.org/medred/medred#> ;
	rdfs:label "ArmList"@en ;
	rdfs:seeAlso :Arm , :Study .
# 
# http://w3id.org/medred/medred#CaseReportForm

:CaseReportForm a owl:Class ;
	rdfs:subClassOf :Instrument ;
	rdfs:comment "A CaseReportForm is a tool used for a clinical study to collect data from each participating subject"@en ;
	rdfs:isDefinedBy <http://w3id.org/medred/medred#> ;
	rdfs:label "CaseReportForm"@en .
# 
# http://w3id.org/medred/medred#Choice

:Choice a owl:Class ;
	rdfs:comment "Each Choice corresponds to a possible answer to a given Question"@en ;
	rdfs:isDefinedBy <http://w3id.org/medred/medred#> ;
	rdfs:label "Choice"@en ;
	rdfs:seeAlso :ChoiceList .
# 
# http://w3id.org/medred/medred#ChoiceList

:ChoiceList a owl:Class ;
	owl:equivalentClass _:genid10 .

_:genid10 a owl:Restriction ;
	owl:onProperty _:genid11 .

_:genid11 owl:inverseOf :hasChoices .

_:genid10 owl:someValuesFrom :Question .

:ChoiceList rdfs:subClassOf rdf:List ;
	rdfs:comment "The ChoiceList corresponds to a list of Choice items for a given Question"@en ;
	rdfs:isDefinedBy <http://w3id.org/medred/medred#> ;
	rdfs:label "ChoiceList"@en .
# 
# http://w3id.org/medred/medred#EventList

:EventList a owl:Class ;
	rdfs:subClassOf rdf:List ;
	rdfs:comment "An EventList is an ordered list of Event elements for a study that is carried out over a long period of time."@en ;
	rdfs:isDefinedBy <http://w3id.org/medred/medred#> ;
	rdfs:label "EventList"@en ;
	rdfs:seeAlso :Event , :Study .
# 
# http://w3id.org/medred/medred#Information

:Information a owl:Class ;
	rdfs:subClassOf :Item ;
	rdfs:comment "Information corresponds to an instrument item that holds an information for the subject"@en ;
	rdfs:isDefinedBy <http://w3id.org/medred/medred#> ;
	rdfs:label "Information"@en .
# 
# http://w3id.org/medred/medred#Instrument

:Instrument a owl:Class ;
	rdfs:subClassOf disco:Instrument , prov:Plan ;
	owl:disjointWith :Observation ;
	rdfs:comment "An Instrument represents a data acquisition tool for a medical study, e.g. a questionnaire, survey, assessment, etc."@en ;
	rdfs:isDefinedBy <http://w3id.org/medred/medred#> ;
	rdfs:label "Instrument"@en .
# 
# http://w3id.org/medred/medred#InstrumentList

:InstrumentList a owl:Class ;
	rdfs:subClassOf rdf:List ;
	rdfs:comment "An InstrumentList is an ordered sequence of Instruments, for a given study."@en ;
	rdfs:isDefinedBy <http://w3id.org/medred/medred#> ;
	rdfs:label "InstrumentList"@en ;
	rdfs:seeAlso :Instrument , :Study .
# 
# http://w3id.org/medred/medred#Item

:Item a owl:Class ;
	rdfs:subClassOf p-plan:Step , _:genid12 .

_:genid12 a owl:Restriction ;
	owl:onProperty dcterms:title ;
	owl:someValuesFrom xsd:string .

:Item rdfs:comment "An Item is a step of an Instrument"@en ;
	rdfs:isDefinedBy <http://w3id.org/medred/medred#> ;
	rdfs:label "Item"@en .
# 
# http://w3id.org/medred/medred#ItemList

:ItemList a owl:Class ;
	rdfs:subClassOf rdf:List ;
	rdfs:comment "The ItemList is a list of Item elements"@en ;
	rdfs:isDefinedBy <http://w3id.org/medred/medred#> ;
	rdfs:label "ItemList"@en .
# 
# http://w3id.org/medred/medred#LongitudinalStudy

:LongitudinalStudy a owl:Class ;
	rdfs:subClassOf :Study ;
	rdfs:comment "A LongitudinalStudy is a study that invloves the repeated observation of data and variables over a period of time"@en ;
	rdfs:isDefinedBy <http://w3id.org/medred/medred#> ;
	rdfs:label "LongitudinalStudy"@en ;
	rdfs:seeAlso disco:Study , :Study .
# 
# http://w3id.org/medred/medred#Observation

:Observation a owl:Class ;
	rdfs:subClassOf p-plan:Entity ;
	rdfs:comment "An Observation is a clinical data element corresponding to an Item in the scope of an Instrument. Observations may include answers to questions, recordings related to a variable, computations effectuated, etc."@en ;
	rdfs:isDefinedBy <http://w3id.org/medred/medred#> ;
	rdfs:label "Observation"@en ;
	rdfs:seeAlso :Instrument , :Item .
# 
# http://w3id.org/medred/medred#Operation

:Operation a owl:Class ;
	rdfs:subClassOf :Item ;
	rdfs:comment "An Operation is an Instrument item that results of a computation, or generated form other items"@en ;
	rdfs:isDefinedBy <http://w3id.org/medred/medred#> ;
	rdfs:label "Operation"@en .
# 
# http://w3id.org/medred/medred#Question

:Question a owl:Class ;
	rdfs:subClassOf disco:Question , :Item ;
	rdfs:comment "A Question is an Instrument item consisting of an inquiry or query to a subject"@en ;
	rdfs:isDefinedBy <http://w3id.org/medred/medred#> ;
	rdfs:label "Question"@en .
# 
# http://w3id.org/medred/medred#Questionnaire

:Questionnaire a owl:Class ;
	rdfs:subClassOf :Instrument ;
	rdfs:comment "A Questionnaire is an Instrument that consists fo different questions made to the subject"@en ;
	rdfs:isDefinedBy <http://w3id.org/medred/medred#> ;
	rdfs:label "Questionnaire"@en .
# 
# http://w3id.org/medred/medred#Section

:Section a owl:Class ;
	rdfs:subClassOf p-plan:MultiStep , :Item ;
	rdfs:comment "A Section is an Instrument item that regroups a subset of Items"@en ;
	rdfs:isDefinedBy <http://w3id.org/medred/medred#> ;
	rdfs:label "Section"@en .
# 
# http://w3id.org/medred/medred#Study

:Study a owl:Class ;
	rdfs:subClassOf disco:Study , prov:Entity ;
	rdfs:comment "A Study is a medical research investigation composed of several instruments"@en ;
	rdfs:isDefinedBy <http://w3id.org/medred/medred#> ;
	rdfs:label "Study"@en ;
	rdfs:seeAlso disco:Study .
# 
# http://w3id.org/medred/medred#StudyEvent

:StudyEvent a owl:Class ;
	rdfs:subClassOf p-plan:Entity ;
	rdfs:comment "A StudyEvent is a planned event within a study (e.g. longitudinal), which will occur at a given time point, and will include a subset of the planned instruments."@en ;
	rdfs:isDefinedBy <http://w3id.org/medred/medred#> ;
	rdfs:label "StudyEvent"@en ;
	rdfs:seeAlso disco:Study , :Study .
# 
# http://www.w3.org/1999/02/22-rdf-syntax-ns#List

rdf:List a owl:Class .
# 
# http://www.w3.org/2000/01/rdf-schema#Datatype

rdfs:Datatype a owl:Class .
# 
# 
# 
# #################################################################
# #
# #    Individuals
# #
# #################################################################
# 
# 
# http://w3id.org/medred/medred#

<http://w3id.org/medred/medred#> a owl:NamedIndividual , <http://purl.org/vocommons/voaf#Vocabulary> .
# 
# http://www.w3.org/1999/02/22-rdf-syntax-ns#nil

rdf:nil a owl:NamedIndividual .
# 
# Generated by the OWL API (version 4.2.5.20160517-0735) https://github.com/owlcs/owlapi
